Prove that the f orbital is subset of combine f g orbital

AutLinOrd/CombineAt.lean
@@ -1,5 +1,4 @@
-import AutLinOrd.NonDecrAt
-import AutLinOrd.OrbitalAt
+import AutLinOrd.OrbitalAtNonDecr
 
 variable {α : Type*} [LinearOrder α]
 
@@ -9,86 +8,174 @@ variable {α : Type*} [LinearOrder α]
   `x` is the union of that of `f` and `g`.
 -/
 noncomputable def combine_at (f g : α ≃o α) (x : α) : α ≃o α :=
-  (orbital_at (non_decr_at f x) x).trans (orbital_at (non_decr_at g x) x)
+  (orbital_at_non_decr f x).trans (orbital_at_non_decr g x)
 
 /--
   For any `y`, we have that `y ≤ (combine_at f g x) y`.
 -/
 theorem not_decr_combine_at (f g : α ≃o α) (x y : α) :
     y ≤ (combine_at f g x) y := by
-  by_cases h : y ∈ elem_orbital (non_decr_at f x) x
-  · by_cases h2 : (non_decr_at f x) y ∈ elem_orbital (non_decr_at g x) x
-    <;> simp [combine_at, orbital_at, h, h2]
-    · have : y ≤ non_decr_at f x y := mem_elem_orbital_non_decr h
-      have : (non_decr_at f x) y ≤ non_decr_at g x ((non_decr_at f x) y) :=
-        mem_elem_orbital_non_decr h2
-      order
-    · exact mem_elem_orbital_non_decr h
-  · by_cases h2 : y ∈ elem_orbital (non_decr_at g x) x
-    <;> simp [combine_at, orbital_at, h, h2]
-    · exact mem_elem_orbital_non_decr h2
+  rw [combine_at]
+  transitivity (orbital_at_non_decr f x) y
+  <;> exact non_decr_orbital_at_non_decr
 
 /--
   For any `y` in the orbital of `x` under `f`,
-  `f y ≤ (combine_at f g x) y`.
+  `(orbital_at_non_decr f x) y ≤ (combine_at f g x) y`.
 -/
-theorem f_le_combine_at {f : α ≃o α} (g : α ≃o α) {x y : α}
-    (y_mem : y ∈ elem_orbital f x) : f y ≤ (combine_at f g x) y := by
-  rw [non_decr_eq_elem_orbital] at y_mem
-  by_cases h2 : (non_decr_at f x) y ∈ elem_orbital (non_decr_at g x) x
-  <;> simp [combine_at, orbital_at, y_mem, h2]
-  · have : f y ≤ (non_decr_at f x) y := mem_elem_orbital_image_non_decr y_mem
-    have : (non_decr_at f x) y ≤ (non_decr_at g x) ((non_decr_at f x) y) :=
-      mem_elem_orbital_non_decr h2
-    order
-  · exact mem_elem_orbital_image_non_decr y_mem
+theorem f_le_combine_at {f : α ≃o α} (g : α ≃o α) {x y : α} :
+    orbital_at_non_decr f x y ≤ (combine_at f g x) y := by
+  rw [combine_at]
+  exact non_decr_orbital_at_non_decr
 
-theorem in_or_above_orbital {f g : α ≃o α} {x y : α}
-    (y_mem : y ∈ elem_orbital f x) (z : ℤ) :
-    (((combine_at f g x ^ z) y) ∈ elem_orbital f x) ∨
-    (∀t ∈ elem_orbital f x, t < (combine_at f g x ^ z) y) := by
-  by_cases h : (((combine_at f g x ^ z) y) ∈ elem_orbital f x)
-  · left
-    trivial
-  · right
-    intro t ht
-    by_contra!
-    absurd h
-    simp only [mem_elem_orbital_iff]
-    constructor
-    · have : y ≤ (combine_at f g x) y := not_decr_combine_at f g x y
-      rw [mem_elem_orbital_iff] at y_mem
-      obtain ⟨⟨l, hl⟩, ⟨u, hu⟩⟩ := y_mem
-      use l
-      have : (combine_at f g x) y ≤  (combine_at f g x ^ z) y := by exact?
+/--
+  For any `y` in the orbital of `x` under `f`,
+  `(orbital_at_non_decr f x) y ≤ (combine_at f g x) y`.
+-/
+theorem inv_f_ge_combine_at {f : α ≃o α} (g : α ≃o α) {x y : α} :
+    (combine_at f g x).symm y ≤ (orbital_at_non_decr f x).symm y := by
+  rw [combine_at]
+  simp only [OrderIso.symm_trans_apply, map_le_map_iff]
+  exact inv_non_decr_orbital_at_non_decr
 
+/--
+  For any `y` in the orbital of `x` under `f`,
+  `(orbital_at_non_decr g x) y ≤ (combine_at f g x) y`.
+-/
+theorem g_le_combine_at {g : α ≃o α} (f : α ≃o α) {x y : α} :
+    orbital_at_non_decr g x y ≤ (combine_at f g x) y := by
+  simp only [combine_at, OrderIso.trans_apply, map_le_map_iff]
+  exact non_decr_orbital_at_non_decr
 
-
-theorem pow_f_le_combine_at {f g : α ≃o α} {x y : α}
-    (y_mem : y ∈ elem_orbital f x) (z : ℤ) :
-    (f^z) y ≤ ((combine_at f g x)^z) y := by
-  induction z with
-  | hz => simp
-  | hp i ih =>
+/--
+  For any `y` and natural number `n`,
+  `(orbital_at_non_decr f x)^n y ≤ (combine_at f g x)^n y`.
+-/
+theorem pow_f_le_combine_at {f g : α ≃o α} {x y : α} (n : ℕ) :
+    ((orbital_at_non_decr f x)^n) y ≤ ((combine_at f g x)^n) y := by
+  induction n with
+  | zero => simp
+  | succ i ih =>
     norm_cast at ih ⊢
-    simp [add_comm i, ←add_pows_n]
-    have : f ((f^i) y) ≤ f ((combine_at f g x ^ i) y) :=
-      OrderIso.GCongr.orderIso_apply_le_apply f ih
-    by_cases h : (combine_at f g x ^ i) y ∈ elem_orbital f x
-    · have := f_le_combine_at g h
-      order
-    · conv =>
-        enter [2, 1]
-        simp [combine_at]
-      simp
-      rw [non_decr_eq_elem_orbital] at h
-      have := orbital_at_not_mem_orbital h
-      simp [this]
-  | hn i _ =>
+    simp only [add_comm i, ← add_pows_n, pow_one, combine_at, OrderIso.trans_apply]
+    transitivity (orbital_at_non_decr f x) ((combine_at f g x ^ i) y)
+    · simp only [map_le_map_iff, ih]
+    · exact non_decr_orbital_at_non_decr
 
-theorem f_in_combine_maps (f g : α ≃o α) (x y : α)
+/--
+  For any `y` and natural number `n`,
+  `(combine_at f g x)^(-n) y ≤ (orbital_at_non_decr f x)^(-n) y`.
+-/
+theorem pow_f_inv_ge_combine_at {f g : α ≃o α} {x y : α} (n : ℕ) :
+    ((combine_at f g x)^(-n : ℤ)) y ≤ ((orbital_at_non_decr f x)^(-n : ℤ)) y := by
+  induction n with
+  | zero => simp
+  | succ n ih =>
+    simp only [zpow_neg, zpow_natCast, Nat.cast_add, Nat.cast_one,
+      neg_add_rev, Int.reduceNeg, ←add_pows, zpow_one] at ih ⊢
+    calc (combine_at f g x).symm ((combine_at f g x ^ n)⁻¹ y)
+    _ ≤ (orbital_at_non_decr f x).symm ((combine_at f g x ^ n)⁻¹ y) :=
+      inv_f_ge_combine_at g
+    _ ≤ (orbital_at_non_decr f x).symm ((orbital_at_non_decr f x ^ n)⁻¹ y) := by
+      simp only [map_le_map_iff, ih]
+
+/--
+  If there exists an integer `z` such that
+  `(orbital_at_non_decr f x)^z x ≤ y`, then
+  there exists an integer `l` such that
+  `(combine_at f g x)^l x ≤ y`.
+-/
+theorem pow_f_le_pow_combine_le {f g : α ≃o α} {x y : α} {z : ℤ}
+    (pow_f_le : ((orbital_at_non_decr f x)^z) x ≤ y) :
+    ∃l : ℤ, ((combine_at f g x)^l) x ≤ y := by
+  cases z with
+  | ofNat n =>
+    simp only [Int.ofNat_eq_coe, zpow_natCast] at pow_f_le
+    use 0
+    simp only [zpow_zero, RelIso.coe_one, id_eq]
+    transitivity (orbital_at_non_decr f x ^ n) x
+    · exact pow_non_decr_orbital_at_non_decr
+    · exact pow_f_le
+  | negSucc n =>
+    simp only [zpow_negSucc] at pow_f_le
+    use Int.negSucc n
+    simp only [zpow_negSucc]
+    transitivity (orbital_at_non_decr f x ^ (n + 1))⁻¹ x
+    · exact pow_f_inv_ge_combine_at (n+1)
+    · exact pow_f_le
+
+/--
+  If there exists an integer `z` such that
+  `y ≤ (orbital_at_non_decr f x)^z x`, then
+  there exists an integer `u` such that
+  `y ≤ (combine_at f g x)^u x`.
+-/
+theorem pow_f_ge_combine_ge {f g : α ≃o α} {x y : α} {z : ℤ}
+    (pow_f_ge : y ≤ ((orbital_at_non_decr f x)^z) x) :
+    ∃u : ℤ, y ≤ ((combine_at f g x)^u) x := by
+  cases z with
+  | ofNat n =>
+    simp only [Int.ofNat_eq_coe, zpow_natCast] at pow_f_ge
+    use n
+    transitivity (orbital_at_non_decr f x ^ n) x
+    · exact pow_f_ge
+    · simp only [zpow_natCast]
+      exact pow_f_le_combine_at n
+  | negSucc n =>
+    simp at pow_f_ge
+    use 0
+    simp only [zpow_zero, RelIso.coe_one, id_eq]
+    transitivity (orbital_at_non_decr f x ^ (n + 1))⁻¹ x
+    · exact pow_f_ge
+    · exact pow_inv_non_decr_orbital_at_non_decr
+
+/--
+  If there exists a `y` such that
+  `(orbital_at_non_decr f x) x = y`,
+  then there exists an integer `l` such that
+  `(combine_at f g x)^l x ≤ y`.
+-/
+theorem f_fix_combine_le {f g : α ≃o α} {x y : α}
+    (fix : (orbital_at_non_decr f x) x = y) :
+    ∃l : ℤ, ((combine_at f g x)^l) x ≤ y := by
+  use 0
+  simp only [zpow_zero, RelIso.coe_one, id_eq]
+  transitivity (orbital_at_non_decr f x) x
+  · exact non_decr_orbital_at_non_decr
+  · exact fix.le
+
+/--
+  If there exists a `y` such that
+  `(orbital_at_non_decr f x) x = y`,
+  then there exists an integer `u` such that
+  `y ≤ (combine_at f g x)^u x`.
+-/
+theorem f_fix_combine_ge {f g : α ≃o α} {x y : α}
+    (fix : (orbital_at_non_decr f x) x = y) :
+    ∃u : ℤ, y ≤ ((combine_at f g x)^u) x := by
+  use 1
+  simp
+  transitivity (orbital_at_non_decr f x) x
+  · exact fix.symm.le
+  · exact non_decr_orbital_at_non_decr
+
+/--
+  If `y` is in the orbital of `x` under `f`,
+  then `y` is in the orbital of `x` under `combine_at f g x`.
+-/
+theorem f_in_combine_map {f : α ≃o α} (g : α ≃o α) {x y : α}
     (y_mem : y ∈ elem_orbital f x) : y ∈ elem_orbital (combine_at f g x) x := by
-  rw [non_decr_eq_elem_orbital, ←orbital_at_eq_orbital,
-    mem_elem_orbital_strong_iff] at y_mem
-  obtain fix | incr | decr := y_mem
-  · simp only [mem_elem_orbital_iff, combine_at, fix]
+  rw [orbital_at_non_decr_orbital_eq, mem_elem_orbital_strong_iff] at y_mem
+  obtain fix | ⟨z, z_le, lt_z⟩ | ⟨z, le_z, z_lt⟩ := y_mem
+  · simp only [combine_at, mem_elem_orbital_iff]
+    constructor
+    · exact f_fix_combine_le fix
+    · exact f_fix_combine_ge fix
+  · simp only [mem_elem_orbital_iff]
+    constructor
+    · exact pow_f_le_pow_combine_le z_le
+    · exact pow_f_ge_combine_ge lt_z.le
+  · simp [mem_elem_orbital_iff]
+    constructor
+    · exact pow_f_le_pow_combine_le le_z
+    · exact pow_f_ge_combine_ge z_lt.le
